src/Analyses/Relational/Rel_Order_Local.thy
@@ -1,5 +1,5 @@
 theory Rel_Order_Local
-  imports Rel_Order_Domain "Voblint_Framework.Oracle_Local_Spec"
+  imports Rel_Order_Domain
 begin
 
 section \<open>The order carrier as a component that asks\<close>
@@ -20,65 +20,96 @@ subsection \<open>Answering queries from the order\<close>
 text \<open>
   A pair \<open>(x, y)\<close> means \<open>s x \<le> s y\<close>. It therefore decides \<open>x <= y\<close> and
   \<open>y >= x\<close> as true, \<open>y < x\<close> and \<open>x > y\<close> as false, and with the reverse pair
-  also \<open>x == y\<close> as true and \<open>x != y\<close> as false. Every other query is answered
-  with \<open>UNIV\<close>, the claim that holds of every store.
+  also \<open>x == y\<close> as true and \<open>x != y\<close> as false. A comparison evaluates to \<open>1\<close>
+  when true and \<open>0\<close> when false, so the answers are \<open>[1,1]\<close> and \<open>[0,0]\<close>. Every
+  other query is answered with \<open>\<top>\<close>, the claim that holds of every store.
 \<close>
 
-fun rel_qry :: "relc \<Rightarrow> query \<Rightarrow> bool set" where
-  "rel_qry d (EvalBool e) =
+text \<open>\<open>rel_le d a b\<close> holds when \<open>a\<close> and \<open>b\<close> are variables whose order \<open>d\<close> records.\<close>
+
+fun var_of :: "exp \<Rightarrow> vname option" where
+  "var_of (V x) = Some x"
+| "var_of _ = None"
+
+definition rel_le :: "relc \<Rightarrow> exp \<Rightarrow> exp \<Rightarrow> bool" where
+  "rel_le d a b =
+     (case (var_of a, var_of b) of (Some x, Some y) \<Rightarrow> relc_has x y d | _ \<Rightarrow> False)"
+
+definition rel_eval :: "relc \<Rightarrow> exp \<Rightarrow> ivl" where
+  "rel_eval d e =
      (case e of
-        LessEq (V x) (V y) \<Rightarrow> if relc_has x y d then {True} else UNIV
-      | GreaterEq (V y) (V x) \<Rightarrow> if relc_has x y d then {True} else UNIV
-      | Less (V y) (V x) \<Rightarrow> if relc_has x y d then {False} else UNIV
-      | Greater (V x) (V y) \<Rightarrow> if relc_has x y d then {False} else UNIV
-      | Eq (V x) (V y) \<Rightarrow>
-          if relc_has x y d \<and> relc_has y x d then {True} else UNIV
-      | NotEq (V x) (V y) \<Rightarrow>
-          if relc_has x y d \<and> relc_has y x d then {False} else UNIV
-      | _ \<Rightarrow> UNIV)"
+        LessEq a b \<Rightarrow> if rel_le d a b then ivl_of_int 1 else \<top>
+      | GreaterEq a b \<Rightarrow> if rel_le d b a then ivl_of_int 1 else \<top>
+      | Less a b \<Rightarrow> if rel_le d b a then ivl_of_int 0 else \<top>
+      | Greater a b \<Rightarrow> if rel_le d a b then ivl_of_int 0 else \<top>
+      | exp.Eq a b \<Rightarrow> if rel_le d a b \<and> rel_le d b a then ivl_of_int 1 else \<top>
+      | NotEq a b \<Rightarrow> if rel_le d a b \<and> rel_le d b a then ivl_of_int 0 else \<top>
+      | _ \<Rightarrow> \<top>)"
+
+fun rel_qry :: "relc \<Rightarrow> answers" where
+  "rel_qry d (EvalInt e) = rel_eval d e"
 
 lemma relc_has_sound: "s \<in> gamma_rel d \<Longrightarrow> relc_has x y d \<Longrightarrow> s x \<le> s y"
   by (cases d) auto
 
-lemma rel_qry_sound: "s \<in> gamma_rel d \<Longrightarrow> truth_holds q (rel_qry d q) s"
-  by (cases q; rename_tac e; case_tac e; simp split: exp.splits)
-     (auto dest: relc_has_sound intro: order_antisym)
+lemma var_of_SomeD: "var_of a = Some x \<Longrightarrow> a = V x"
+  by (cases a) simp_all
+
+lemma rel_le_sound: "s \<in> gamma_rel d \<Longrightarrow> rel_le d a b \<Longrightarrow> \<lbrakk>a\<rbrakk>\<^sub>e s \<le> \<lbrakk>b\<rbrakk>\<^sub>e s"
+  by (auto simp: rel_le_def split: option.splits dest!: var_of_SomeD
+      dest: relc_has_sound)
+
+lemma rel_eval_sound: "s \<in> gamma_rel d \<Longrightarrow> \<lbrakk>e\<rbrakk>\<^sub>e s \<in> gamma_ivl (rel_eval d e)"
+  by (cases e) (auto simp: rel_eval_def top_ivl_def gamma_ivl_top
+      dest: rel_le_sound intro: order_antisym)
+
+lemma rel_qry_sound: "s \<in> gamma_rel d \<Longrightarrow> eval_holds q (rel_qry d q) s"
+  by (cases q) (simp add: rel_eval_sound)
 
 subsection \<open>Learning orders from the oracle\<close>
 
 text \<open>
   At \<open>x = e\<close> the question is asked about the state before the assignment, where
   \<open>e\<close> evaluates to the new value of \<open>x\<close> and every other variable keeps its
-  value. An answer \<open>{True}\<close> to \<open>e <= y\<close> therefore makes \<open>(x, y)\<close> true
+  value. An answer \<open>[1,1]\<close> to \<open>e <= y\<close> therefore makes \<open>(x, y)\<close> true
   afterwards, and \<open>y <= e\<close> makes \<open>(y, x)\<close> true. The candidate partners are the
   variables in \<open>ys\<close>, a parameter so that the construction stays executable.
 \<close>
 
-definition rel_learn ::
-  "(query \<Rightarrow> bool set) \<Rightarrow> vname list \<Rightarrow> vname \<Rightarrow> exp \<Rightarrow> relc \<Rightarrow> relc" where
+definition rel_learn :: "answers \<Rightarrow> vname list \<Rightarrow> vname \<Rightarrow> exp \<Rightarrow> relc \<Rightarrow> relc" where
   "rel_learn ask ys x e d =
      (case d of
         Bot \<Rightarrow> Bot
       | RelC ps \<Rightarrow> RelC (ps
           \<union> set (map (\<lambda>y. (x, y))
-                (filter (\<lambda>y. y \<noteq> x \<and> ask (EvalBool (LessEq e (V y))) = {True}) ys))
+                (filter (\<lambda>y. y \<noteq> x \<and> ivl_const (ask (EvalInt (LessEq e (V y)))) = Some 1) ys))
           \<union> set (map (\<lambda>y. (y, x))
-                (filter (\<lambda>y. y \<noteq> x \<and> ask (EvalBool (LessEq (V y) e)) = {True}) ys))))"
+                (filter (\<lambda>y. y \<noteq> x \<and> ivl_const (ask (EvalInt (LessEq (V y) e))) = Some 1) ys))))"
+
+text \<open>The questions \<open>rel_learn\<close> consults at \<open>x = e\<close>, and nothing elsewhere.\<close>
+
+definition rel_qs :: "vname list \<Rightarrow> edge_action \<Rightarrow> relc \<Rightarrow> query list" where
+  "rel_qs ys a d =
+     (case a of
+        EA_Assign x e \<Rightarrow>
+          concat (map (\<lambda>y. if y = x then []
+                           else [EvalInt (LessEq e (V y)), EvalInt (LessEq (V y) e)]) ys)
+      | _ \<Rightarrow> [])"
 
 lemma rel_learn_sound:
   assumes "s(x := \<lbrakk>e\<rbrakk>\<^sub>e s) \<in> gamma_rel d"
-    and "truth_query.oracle_holds ask s"
+    and "eval_query.oracle_holds ask s"
   shows "s(x := \<lbrakk>e\<rbrakk>\<^sub>e s) \<in> gamma_rel (rel_learn ask ys x e d)"
 proof (cases d)
   case Bot
   with assms(1) show ?thesis by simp
 next
   case (RelC ps)
-  have up: "\<lbrakk>e\<rbrakk>\<^sub>e s \<le> s y" if "ask (EvalBool (LessEq e (V y))) = {True}" for y
-    using truth_query.oracle_holdsD[OF assms(2), of "EvalBool (LessEq e (V y))"] that
+  have up: "\<lbrakk>e\<rbrakk>\<^sub>e s \<le> s y" if "ivl_const (ask (EvalInt (LessEq e (V y)))) = Some 1" for y
+    using eval_holds_constD[OF eval_query.oracle_holdsD[OF assms(2)] that]
     by (simp split: if_splits)
-  have down: "s y \<le> \<lbrakk>e\<rbrakk>\<^sub>e s" if "ask (EvalBool (LessEq (V y) e)) = {True}" for y
-    using truth_query.oracle_holdsD[OF assms(2), of "EvalBool (LessEq (V y) e)"] that
+  have down: "s y \<le> \<lbrakk>e\<rbrakk>\<^sub>e s" if "ivl_const (ask (EvalInt (LessEq (V y) e))) = Some 1" for y
+    using eval_holds_constD[OF eval_query.oracle_holdsD[OF assms(2)] that]
     by (simp split: if_splits)
   show ?thesis
     using assms(1) RelC up down by (auto simp: rel_learn_def)
@@ -90,18 +121,18 @@ definition rel_ret :: "exp option \<Rightarrow> relc \<Rightarrow> relc" where
   "rel_ret eo d = (case eo of None \<Rightarrow> d | Some a \<Rightarrow> forget_relc ret_var d)"
 
 theorem rel_local_component:
-  "oracle_component truth_holds
-     (\<lambda>ask d. d)
-     (\<lambda>ask x e d. rel_learn ask ys x e (forget_relc x d))
-     (\<lambda>ask sc x d. forget_relc x d)
-     (\<lambda>ask b pol d. branch_step_rel b pol d)
-     (\<lambda>ask p d. d)
-     (\<lambda>ask eo p d. rel_ret eo d)
+  "sound_local_dg_spec rel_qry
+     (\<lambda>A d. d)
+     (\<lambda>A x e d. rel_learn A ys x e (forget_relc x d))
+     (\<lambda>A sc x d. forget_relc x d)
+     (\<lambda>A b pol d. branch_step_rel b pol d)
+     (\<lambda>A p d. d)
+     (\<lambda>A eo p d. rel_ret eo d)
      (\<lambda>ci d. [(d, top_relc)])
-     (\<lambda>ask ev d. d)
+     (\<lambda>A ev d. d)
      (\<lambda>ci dc de. dc)
      (\<lambda>ci d de. top_relc)
-     gamma_rel \<G> rel_qry"
+     gamma_rel \<G>"
 proof (unfold_locales, goal_cases)
   case (1 d d')
   then show ?case by (rule gamma_rel_mono)
